WIP on preservation proof for L3->L4.

theories/L4_deBruijn/L3_to_L4.v
@@ -10,7 +10,7 @@ Opaque N.sub.
 Require Import L3.program.
 
 Require L3.L3.
-Module L3eval := L3.wndEval.
+Module L3eval := L3.wcbvEval.
 Module L3t := L3.term.
 Module L3U := L3.unaryApplications.
 Require Import L4.expression.
@@ -89,27 +89,491 @@ End TermTranslation.
 Definition translate (e : env) t :=
   trans e 0 t.
 
+Definition translate_entry x acc :=
+  match x with
+  | (s, ecTrm t) =>
+    let t' := translate acc t in
+    (s, t') :: acc
+  | (s, ecTyp _) => acc
+  end.
+
+Definition translate_entry_aux x acc : option (string * exp) :=
+  match x with
+  | (s, ecTrm t) =>
+    let t' := translate acc t in
+    Some (s, t')
+  | (s, ecTyp _) => None
+  end.
+
+Definition translate_env_aux (e : environ) (k : env) : env :=
+  fold_right translate_entry k e.
+
 Definition translate_env (e : environ) : env :=
-  fold_right
-    (fun x acc => match x with
-               | (s, ecTrm t) =>
-                 let t' := translate acc t in
-                   (s, t') :: acc
-               | (s, ecTyp _) => acc
-               end) [] e.
+  translate_env_aux e [].
 
 Definition mkLets (e : env) (t : exp) :=
-  fold_left (fun acc (x : string * exp) => let (s, t) := x in Let_e t acc) e t.
+  fold_left (fun acc (x : string * exp) => Let_e (snd x) acc) e t.
+
+Definition let_entry acc (a : string * envClass) e :=
+  match a with
+  | (s, ecTrm t) =>
+    let t' := translate acc t in
+    Let_e t' e
+  | (s, ecTyp _) => e
+  end.
+
+Lemma mkLets_translate a e t :
+  mkLets (translate_env (a :: e)) t =
+  mkLets (translate_env e) (let_entry (translate_env e) a t).
+Proof.
+  now destruct a as [s [trm|ty]].
+Qed.
 
 Definition translate_program (e : environ) (t : L3t.Term) : exp :=
   let e' := translate_env e in
     mkLets e' (translate e' t).
-              
-Theorem translate_correct (e : environ) (t t' : L3t.Term) :
-  L3eval.wndEval e t t' -> (* small step non-deterministic *)
-  eval (translate_program e t) (translate_program e t'). (* big-step deterministic *)
+
+Definition subst_env_aux e n (t : exp) :=
+  fold_left
+    (fun t (x : string * exp) => t{n ::= snd x})
+    e t.
+
+Definition subst_env e (t : exp) := subst_env_aux e 0 t.
+
+Definition subst_entry (a : string * envClass) acc (e : exp) :=
+  match a with
+  | (s, ecTrm t) =>
+    let t' := translate acc t in
+      e{0 ::= t'}
+  | (s, ecTyp _) => e
+  end.
+
+Lemma subst_env_tr a e k t :
+  subst_env (translate_entry a (translate_env_aux e k)) t =
+  subst_env (translate_env_aux e k)
+            (subst_entry a (translate_env_aux e k) t).
 Proof.
-  induction 1. simpl. red in H.
+  destruct a as [s [trm|ty]]; cbn; reflexivity.
+Qed.
+
+Lemma translate_env_aux_snoc e a acc :
+  translate_env_aux (e ++ [a]) acc =
+  translate_env_aux e (translate_entry a acc). 
+Proof.
+  unfold translate_env_aux.
+  rewrite fold_right_app; simpl. reflexivity.
+Qed.
+
+Definition build_subst_fn :=
+  (fun (x : string * envClass) acc =>
+                let '(acc, k) := acc in
+                match translate_entry_aux x k with
+                | Some r => (r :: acc, r :: k)
+                | None => (acc, k)
+                end).
+
+Lemma snd_build_subst_fn a k :
+  snd (build_subst_fn a k) = translate_entry a (snd k).
+Proof.
+  destruct k as [acc k].
+  destruct a as [s [trm|ty]]; reflexivity.
+Qed.
+
+Definition build_subst_aux e acc :=
+  fold_right build_subst_fn acc e.
+
+Definition build_subst e k :=
+  build_subst_aux e ([], k).
+
+Definition substl l (e : exp) :=
+  fold_left (fun t e => t{0 ::= e}) l e.
+
+Lemma substl_app l l' e : substl l (substl l' e) = substl (l' ++ l) e.
+Proof.
+  revert l e; induction l'; intros l e; simpl.
+  - reflexivity.
+  - rewrite IHl'.
+    reflexivity.
+Qed.
+
+Definition subst_entries e k (t : exp) :=
+  let s := build_subst e k in
+  substl (map snd (fst s)) t.
+
+Lemma subst_env_translate_env e a k t :
+  subst_env (translate_env_aux (a :: e) k) t =
+  subst_env (translate_env_aux e k) (subst_entry a (translate_env_aux e k) t).
+Proof.
+  destruct a as [s [trm | ty]] ; simpl.
+  + reflexivity.
+  + reflexivity.
+Qed.
+
+Lemma build_subst_lemma a e' e :
+  build_subst (a :: e') e =
+  build_subst_fn a (build_subst e' e).
+Proof. reflexivity. Qed.
+
+Ltac case_call f :=
+  let call := fresh "call" in
+  remember f as call; destruct call.
+
+Lemma build_subst_aux_lemma e' e'' acc :
+  build_subst_aux (e'' ++ e') acc =
+  build_subst_aux e'' (build_subst_aux e' acc).
+Proof.
+  revert e'' acc; induction e' as [ |x e'] using rev_ind; intros e'' acc.
+  simpl.
+  - now rewrite !app_nil_r. 
+  - specialize (IHe' e'').
+    unfold build_subst_aux.
+    now rewrite fold_right_app.
+Qed.
+
+Definition build_subst_app e e' e'' :=
+  let '(s, k) := build_subst e' e in
+  let '(s', k') := build_subst e'' k in
+  (s' ++ s, k').
+
+Lemma build_subst_lemma' e' e'' e :
+  build_subst (e'' ++ e') e = build_subst_app e e' e''.
+Proof.
+  unfold build_subst, build_subst_app in *.
+  case_call (build_subst e' e).
+  case_call (build_subst e'' e0).
+  unfold build_subst, build_subst_app in *.
+  rewrite build_subst_aux_lemma.
+  rewrite <- Heqcall.
+  clear Heqcall.
+  revert l0 e1 e0 Heqcall0. clear.
+  induction e''; simpl; intros.
+  + injection Heqcall0; intros; subst. 
+    reflexivity.
+  + case_call (build_subst_aux e'' ([], e0)).
+    specialize (IHe'' _ _ _ Heqcall).
+    rewrite IHe''.
+    simpl in *.
+    case_call (translate_entry_aux a e);
+    injection Heqcall0; intros; subst;
+    reflexivity.
+Qed.
+
+Lemma translate_env_aux_build_subst e k :
+  translate_env_aux e k = snd (build_subst e k).
+Proof.
+  revert k; induction e using rev_ind; intros; try reflexivity.
+  unfold translate_env_aux, build_subst, build_subst_aux in *.
+  simpl.
+  rewrite !fold_right_app.
+  rewrite IHe.
+  simpl.
+  unfold translate_entry, translate_entry_aux.
+  destruct x as [s [trm|ty]]; simpl; try reflexivity.
+  generalize ((s, translate k trm) :: k).
+  clear. induction e; simpl; intros.
+  + reflexivity.
+  + rewrite !snd_build_subst_fn.
+    f_equal. apply IHe.
+Qed.
+  
+  
+Lemma subst_entries_comm e e' k t :
+  subst_entries e k (subst_entries e' (snd (build_subst e k)) t) =
+  subst_entries (e' ++ e) k t.
+Proof.
+  unfold subst_entries.
+  case_call (build_subst e k).
+  case_call (build_subst e' e0).
+  pose proof (build_subst_lemma' e e' k).
+  unfold build_subst_app in H.
+  rewrite <- Heqcall in *.
+  rewrite <- Heqcall0 in H.
+  rewrite H, substl_app. f_equal.
+  simpl.
+  f_equal. now rewrite <- Heqcall0; simpl; rewrite map_app.
+Qed.
+
+Lemma subst_env_translate_env_k e k t :
+  subst_env (translate_env_aux e k) t =
+  subst_env k (subst_entries e k t).
+Proof.
+  revert k t.
+  induction e.
+  - reflexivity.
+  - intros. simpl.
+    rewrite subst_env_tr.
+    rewrite IHe.
+    f_equal.
+    rewrite translate_env_aux_build_subst.
+    replace (subst_entry a (snd (build_subst e k)) t) with
+    (subst_entries [a] (snd (build_subst e k)) t).
+    rewrite subst_entries_comm. reflexivity.
+    destruct a as [s [trm|ty]]; reflexivity.
+Qed.
+
+
+Lemma mkLets_app e e' t : mkLets (e ++ e') t =
+                          mkLets e' (mkLets e t).
+Proof.
+  revert t; induction e; intros.
+  - simpl. reflexivity.
+  - simpl. rewrite IHe.
+    reflexivity.
+Qed.
+
+Lemma build_subst_aux_app e e' :
+  snd (build_subst_aux e e') = snd (build_subst_aux e ([], snd e')).
+Proof.
+  induction e; simpl.
+  - reflexivity.
+  - case_call (build_subst_aux e e').
+    case_call (build_subst_aux e ([], snd e')).
+    simpl in *. subst.
+    destruct a as [s [trm|ty]].
+    reflexivity.
+    reflexivity.
+Qed.
+
+Lemma build_subst_aux_app' e e' :
+  snd (build_subst_aux e e') = fst (build_subst_aux e ([], snd e')) ++ snd e'.
+Proof.
+  revert e'; induction e; simpl; intros.
+  + reflexivity.
+  + specialize (IHe e').
+    case_call (build_subst_aux e e').
+    simpl.
+    case_call (build_subst_aux e ([], snd e')).
+    simpl in *. subst e0.
+    destruct a as [s [trm|ty]]; simpl.
+    - f_equal. f_equal.
+      pose (build_subst_aux_app e e').
+      rewrite <- Heqcall, <- Heqcall0 in e0.
+      simpl in e0. subst e1. reflexivity.
+    - reflexivity.
+Qed.
+
+Lemma build_subst_fst_snd e : snd (build_subst e []) = fst (build_subst e []).
+Proof.
+  induction e. reflexivity.
+  simpl.
+  destruct a as [s [trm|ty]];
+  case_call (build_subst e []); simpl in *; subst; reflexivity.
+Qed.  
+                                 
+Lemma translate_env_app e e' :
+  translate_env (e' ++ e) = 
+  (fst (build_subst e' (translate_env e))) ++ translate_env e.
+Proof.
+  unfold translate_env.
+  rewrite !translate_env_aux_build_subst.
+  unfold build_subst at 1.
+  rewrite build_subst_aux_lemma, build_subst_aux_app'.
+  f_equal.
+Qed.
+
+Lemma mkLets_translate_app e e' t :
+  mkLets (translate_env (e' ++ e)) t =
+  mkLets (translate_env e)
+         (mkLets (fst (build_subst e' (translate_env e))) t).
+Proof.
+  now rewrite <- mkLets_app, translate_env_app.
+Qed.
+
+Lemma mkLets_translate_entry x  t :
+  mkLets (translate_entry x []) t = let_entry [] x t.
+Proof.
+  destruct x as [s [trm|ty]]. simpl. reflexivity.
+  simpl. reflexivity.
+Qed.
+
+Definition sbst_env_aux (u : exp) (e : env) acc : N * env :=
+  fold_right (fun s acc =>
+                let '(n, l) := acc in
+                (n+1, (fst s, (snd s){n ::= u}) :: l))
+             acc e.
+
+Definition sbst_env (u : exp) (n : N) (e : env) : N * env :=
+  sbst_env_aux u e (n, []).
+
+Lemma sbst_env_app e k l acc : sbst_env_aux e (k ++ l) acc =
+                               sbst_env_aux e k (sbst_env_aux e l acc).
+Proof.
+  now unfold sbst_env_aux; rewrite fold_right_app. 
+Qed.
+
+Lemma fst_sbst_env_aux e k acc :
+  fst (sbst_env_aux e k acc) = fst (sbst_env_aux e k (fst acc, [])).
+Proof.
+  induction k; simpl.
+  - reflexivity.
+  - case_call (sbst_env_aux e k acc).
+    simpl in *. 
+    case_call (sbst_env_aux e k (fst acc, [])).
+    subst n; simpl. reflexivity.
+Qed.
+    
+Lemma snd_sbst_env_aux e k acc :
+  snd (sbst_env_aux e k acc) =
+  snd (sbst_env_aux e k (fst acc, [])) ++ snd acc.
+Proof.
+  induction k; simpl.
+
+  - reflexivity.
+  - generalize (fst_sbst_env_aux e k acc).
+    case_call (sbst_env_aux e k acc).
+    simpl in *. 
+    case_call (sbst_env_aux e k (fst acc, [])).
+    subst e0; simpl.
+    f_equal. f_equal.
+    simpl in *.
+    now intros ->.
+Qed.
+
+
+Lemma sbst_lets (e : exp) (n : N) k t :
+  let k' := (sbst_env e n k) in
+  sbst e n (mkLets k t) = mkLets (snd k') (sbst e (fst k') t).
+Proof.
+  revert n t; induction k using rev_ind; intros.
+  - simpl. reflexivity.
+  - simpl.
+    rewrite mkLets_app.
+    simpl.
+    unfold sbst_env in k'.
+    rewrite IHk.
+    subst k'. rewrite sbst_env_app.
+    rewrite snd_sbst_env_aux.
+    rewrite mkLets_app.
+    rewrite snd_sbst_env_aux.
+    rewrite mkLets_app.
+    unfold mkLets at 2. simpl.
+    f_equal. f_equal.
+    + unfold sbst_env. now rewrite N.add_1_r, N.add_1_l.
+    + unfold sbst_env. rewrite N.add_1_r, N.add_1_l.
+      now setoid_rewrite fst_sbst_env_aux at 2.
+Qed.
+      
+    
+Lemma length_sbst_env e n k : length (snd (sbst_env e n k)) = length k.
+Proof.
+  revert e n; induction k using rev_ind; intros.
+  simpl. reflexivity.
+  unfold sbst_env.
+  rewrite sbst_env_app.
+  simpl.
+  rewrite snd_sbst_env_aux.
+  rewrite !app_length. simpl.
+  unfold sbst_env in IHk. rewrite IHk.
+  reflexivity.
+Qed.
+
+Lemma subst_env_app k x t :
+  let k' := sbst_env (snd x) 0 k in
+  subst_env (k ++ [x]) t =
+  (subst_env (snd k') (sbst (snd x) (fst k') t)).
+Proof.
+  intros.
+  revert t x k'. induction k; intros.
+  - reflexivity.
+  - simpl.
+    subst k'.
+    rewrite IHk.
+    unfold sbst_env.
+    simpl.
+Admitted.
+
+Lemma eval_lets e t t' :
+  eval (subst_env e t) t' ->
+  eval (mkLets e t) t'.
+Proof.
+  revert t t'. pattern e. refine (wf_ind (@length _) _ _ e). clear.
+  simpl. intros k IHk ? ?. destruct k using rev_ind; intros.
+  + simpl. trivial.
+  + simpl. clear IHk0.
+    rewrite mkLets_app.
+    simpl.
+    econstructor. instantiate (v1 := snd x). admit.
+    simpl in IHk.
+    simpl.
+    rewrite sbst_lets.
+    apply IHk.
+    rewrite length_sbst_env, app_length.
+    simpl. omega.
+    rewrite <- subst_env_app. assumption.
+Admitted.
+
+Lemma subst_env_aux_lam e k t :
+  subst_env_aux e k (Lam_e t) = Lam_e (subst_env_aux e (1 + k) t).
+Proof.
+  revert t; induction e; intros; simpl.
+  - reflexivity.
+  - now rewrite IHe.
+Qed.
+
+Definition subst_env_lam e t : subst_env e (Lam_e t) = Lam_e (subst_env_aux e 1 t) :=
+  subst_env_aux_lam e 0 t.
+
+Lemma subst_env_aux_var e k nm t :
+  LookupDfn nm e t ->
+  subst_env_aux (translate_env e) k (Var_e (cst_offset (translate_env e) nm + k)) =
+  subst_env (translate_env e) (translate (translate_env e) t).
+Proof.
+  revert t; induction e; intros; simpl.
+  - inversion H.
+Admitted.
+
+Theorem translate_correct (e : environ) (t t' : L3t.Term) :
+  L3eval.WcbvEval e t t' -> (* small step non-deterministic *)
+  let e' := translate_env e in
+  eval (mkLets e' (translate e' t)) (subst_env e' (translate e' t')). (* big-step deterministic *)
+Proof.
+  cbn. intros H. apply eval_lets.
+  induction H.
+
+  + (* Lambda *)
+    cbn.
+    rewrite subst_env_lam. constructor.
+
+  + (* Prod *)
+    cbn. 
+    admit.
+
+  + unfold translate. (* mutual *)
+    admit.
+
+  + (* Ind *)
+    unfold translate.
+    simpl.
+    admit.
+
+  + (* Sort *)
+    admit.
+
+  + (* Fix *)
+    admit.
+
+  + (* Const *)
+    unfold translate.
+    simpl.
+    (* IH is not strong enough here *)
+    unfold subst_env at 1.
+    erewrite subst_env_aux_var.
+    apply IHWcbvEval. assumption.
+
+  + (* App Lam *)
+    admit.
+
+  + (* LetIn *)
+    admit.
+
+  + (* App Fix *)
+    admit.
+
+  + (* Construct *)
+    admit.
+
+  + (* Case *)
+    admit.
 Admitted.
 
 (** start-to-L4 translations **)
